wip on ClosedComp

src/ClosedComp.v
@@ -8,6 +8,8 @@ Require Closed.
 Require Utopia.
 Require String.
 
+Require Import UntypedFCont.
+
 Module A := Untyped.
 Module B := Closed.
 
@@ -35,12 +37,12 @@ Definition compile (n : nat) (e : A.expr) : B.expr :=
           | e :: es => go n e :: go_list es
           end in
       match e with
-      | A.Var n => 
+      | A.Var n =>
         match n with
         | 0 => B.Arg
         | S n => B.UpVar n
         end
-      | A.Lam body => B.Close (go n body) (close_vars n)
+      | A.Lam body => B.Close (go (S n) body) (close_vars n)
       | A.App e1 e2 => B.Call (go n e1) (go n e2)
       | A.Constr c args => B.Constr c (go_list args)
       | A.Elim ty cases target => B.Elim ty (go_list cases) (go n target)
@@ -58,15 +60,262 @@ Definition compile_cu (cu : list A.expr * list metadata) : list B.expr * list me
   let '(exprs, metas) := cu 
   in (compile_list 0 exprs, metas).
 
-Axiom shift : B.expr -> B.expr.
+Module example.
+  Definition a := A.App (A.App (A.Lam (A.Lam (A.App (A.Var 1) (A.Var 0))))
+                               (A.Lam (A.Var 0)))
+                        (A.Constr Utopia.Ctt []).
 
+  Definition a1 := A.App (A.Lam (A.Lam (A.App (A.Var 1) (A.Var 0))))
+                         (A.Lam (A.Var 0)).
+  Definition ka1 := fun v => Run (Untyped.App v (A.Constr Utopia.Ctt [])) Stop.
+
+  Lemma step_a1 : sstep (Run a Stop) (Run a1 ka1).
+  Proof.
+    constructor.
+    intro.
+    solve_by_inversion.
+  Qed.
+
+
+  Definition a2 := Untyped.Lam (Untyped.App (Untyped.Lam (A.Var 0)) (A.Var 0)).
+  Definition ka2 := ka1.
+
+  Lemma step_a2 : sstep (Run a1 ka1) (Run a2 ka2).
+  Proof.
+    constructor.
+    auto.
+  Qed.
+
+
+  Definition a3 := Untyped.App (Untyped.Lam (Untyped.App (Untyped.Lam (A.Var 0)) (A.Var 0)))
+                               (A.Constr Utopia.Ctt []).
+
+  Lemma step_a3 : sstep (Run a2 ka2) (Run a3 Stop).
+  Proof.
+    constructor.
+  Qed.
+
+
+  Definition a4 := Untyped.App (Untyped.Lam (A.Var 0)) (A.Constr Utopia.Ctt []).
+
+  Lemma step_a4 : sstep (Run a3 Stop) (Run a4 Stop).
+  Proof.
+    constructor.
+    auto.
+  Qed.
+
+
+  Definition a5 := A.Constr Utopia.Ctt [].
+
+  Lemma step_a5 : sstep (Run a4 Stop) (Run a5 Stop).
+  Proof.
+    constructor.
+    auto.
+  Qed.
+
+
+  Lemma step_final : sstep (Run a5 Stop) (Stop a5).
+  Proof.
+    constructor.
+    auto.
+  Qed.
+
+
+
+
+  Definition b := B.Call (B.Call (B.Close (B.Close (B.Call (B.UpVar 0) B.Arg) [B.Arg]) [])
+                                 (B.Close B.Arg []))
+                         (B.Constr Utopia.Ctt []).
+
+
+  Lemma a_b : compile 0 a = b.
+  Proof. auto. Qed.
+
+
+  Definition b1 := B.Call (B.Close (B.Close (B.Call (B.UpVar 0) B.Arg) [B.Arg]) [])
+                          (B.Close B.Arg []).
+  Definition kb1 := fun v => B.Run (B.Call v (B.Constr Utopia.Ctt [])) [] B.Stop.
+
+  Lemma step_b1 : B.sstep (B.Run b [] B.Stop) (B.Run b1 [] kb1).
+  Proof.
+    constructor.
+    intro.
+    solve_by_inversion.
+  Qed.
+
+
+  Definition b2 := B.Close (B.Call (B.UpVar 0) B.Arg) [B.Arg].
+  Definition l2 := [B.Close B.Arg []].
+  Definition kb2 := kb1.
+
+  Lemma step_b2 : B.sstep (B.Run b1 [] kb1) (B.Run b2 l2 kb2).
+  Proof.
+    apply B.SMakeCall; auto.
+  Qed.
+
+
+  Definition b3 := B.Arg.
+  Definition l3 := l2.
+  Definition kb3 := fun v => B.Run (B.Close (B.Call (B.UpVar 0) B.Arg) [v]) l2 kb2.
+
+  Lemma step_b3 : B.sstep (B.Run b2 l2 kb2) (B.Run b3 l3 kb3).
+  Proof.
+    eapply B.SCloseStep with (vs := []); auto.
+    intro. solve_by_inversion.
+  Qed.
+
+
+  Definition b35 := (B.Close B.Arg []).
+  Definition l35 := l3.
+  Definition kb35 := kb3.
+
+  Lemma step_b3point5 : B.sstep (B.Run b3 l3 kb3) (B.Run b35 l35 kb35) .
+  Proof.
+    eapply eq_rect.
+    econstructor. cbn. auto.
+    auto.
+  Qed.
+
+  Definition b4 := (B.Close (B.Call (B.UpVar 0) B.Arg) [B.Close B.Arg []]).
+  Definition l4 := l2.
+  Definition kb4 := kb2.
+
+  Lemma step_b4 : B.sstep (B.Run b35 l35 kb35) (B.Run b4 l4 kb4).
+  Proof.
+    eapply eq_rect.
+    econstructor. cbn. auto.
+    auto.
+  Qed.
+
+
+  Definition b5 := B.Call (B.Close (B.Call (B.UpVar 0) B.Arg) [B.Close B.Arg []])
+                          (B.Constr Utopia.Ctt []).
+
+  Lemma step_b5 :  B.sstep (B.Run b4 l4 kb4) (B.Run b5 [] B.Stop).
+  Proof.
+    econstructor.
+    auto.
+  Qed.
+
+
+  Definition b6 := (B.Call (B.UpVar 0) B.Arg).
+  Definition l6 := [B.Constr Utopia.Ctt []; B.Close B.Arg []].
+
+  Lemma step_b6 : B.sstep (B.Run b5 [] B.Stop) (B.Run b6 l6 B.Stop).
+  Proof.
+    apply B.SMakeCall; auto.
+  Qed.
+
+
+  Definition b7 := B.UpVar 0.
+  Definition l7 := l6.
+  Definition kb7 := fun v => B.Run (B.Call v B.Arg) l6 B.Stop.
+
+  Lemma step_b7 : B.sstep (B.Run b6 l6 B.Stop) (B.Run b7 l7 kb7).
+  Proof.
+    econstructor.
+    intro. solve_by_inversion.
+  Qed.
+
+
+
+  Definition b75 := (B.Close B.Arg []).
+  Definition l75 := l7.
+  Definition kb75 := kb7.
+
+  Lemma step_b75 : B.sstep (B.Run b7 l7 kb7) (B.Run b75 l75 kb75).
+  Proof.
+    eapply eq_rect.
+    constructor.
+    cbn. auto.
+    auto.
+  Qed.
+
+
+  Definition b8 := (B.Call (B.Close B.Arg []) B.Arg).
+  Definition l8 := l6.
+
+  Lemma step_b8 : B.sstep (B.Run b75 l75 kb75) (B.Run b8 l8 B.Stop).
+  Proof.
+    eapply eq_rect.
+    constructor.
+    cbn. auto.
+    auto.
+  Qed.
+
+
+  Definition b9 := B.Arg.
+  Definition l9 := l8.
+  Definition kb9 := fun v => B.Run (B.Call (B.Close B.Arg []) v) l8 B.Stop.
+
+  Lemma step_b9 : B.sstep (B.Run b8 l8 B.Stop) (B.Run b9 l9 kb9).
+  Proof.
+    eapply B.SCallR; auto.
+    intro. solve_by_inversion.
+  Qed.
+
+
+  Definition b95 := (B.Constr Utopia.Ctt []).
+  Definition l95 := l9.
+  Definition kb95 := kb9.
+
+  Lemma step_b95 : B.sstep (B.Run b9 l9 kb9) (B.Run b95 l95 kb9).
+  Proof.
+    eapply eq_rect.
+    econstructor. simpl. auto.
+    auto.
+  Qed.
+
+  Definition b10 := (B.Call (B.Close B.Arg []) (B.Constr Utopia.Ctt [])).
+  Definition l10 := l8.
+
+  Lemma step_b10 : B.sstep (B.Run b95 l95 kb95) (B.Run b10 l10 B.Stop).
+  Proof.
+    eapply eq_rect.
+    econstructor. simpl. auto.
+    auto.
+  Qed.
+
+
+  Definition b11 := B.Arg.
+  Definition l11 := [B.Constr Utopia.Ctt []].
+
+  Lemma step_b11 : B.sstep (B.Run b10 l10 B.Stop) (B.Run b11 l11 B.Stop).
+  Proof.
+    eapply B.SMakeCall; auto.
+  Qed.
+
+
+  Definition b12 := (B.Constr Utopia.Ctt []).
+  Definition l12 := l11.
+
+  Lemma step_b12 : B.sstep (B.Run b11 l11 B.Stop) (B.Run b12 l12 B.Stop).
+  Proof.
+    econstructor.
+    simpl. auto.
+  Qed.
+
+
+  Lemma step_b13 : B.sstep (B.Run b12 l12 B.Stop) (B.Stop b12).
+  Proof.
+    econstructor.
+    auto.
+  Qed.
+End example.
+(*
 Inductive I_expr : list B.expr -> A.expr -> B.expr -> Prop :=
-| IArg : forall l b, nth_error l 0 = Some b -> I_expr l (A.Var 0) b
-| IUpVar : forall l n b, nth_error l (S n) = Some b -> I_expr l (A.Var (S n)) b
-| ILam : forall l a1 b1, 
-    I_expr (B.Arg :: map shift l) a1 b1 -> 
+| IArg l a b :
+    nth_error l 0 = Some b ->
+    I_expr l a b ->
+    I_expr l a B.Arg
+| IUpVar l a b n :
+    nth_error l (S n) = Some b ->
+    I_expr l a b ->
+    I_expr l a (B.UpVar n)
+| ILam n a1 b1 :
+    I_expr (S n) a1 b1 ->
     I_expr l (A.Lam a1) (B.Close b1 (close_vars (length l)))
-| IApp : forall l a1 a2 b1 b2, 
+| IApp : forall l a1 a2 b1 b2,
     I_expr l a1 b1 -> 
     I_expr l a2 b2 -> 
     I_expr l (A.App a1 a2) (B.Call b1 b2)
@@ -100,3 +349,4 @@ Section Preservation.
     forward_simulation (A.semantics prog) (B.semantics tprog).
   Proof.
     eapply forward_simulation_step.
+*)
